Semantic/CC.lean
@@ -6,8 +6,8 @@ import Semantic.CC.Substitution
 
 import Semantic.CC.TypeSystem
 
-import Semantic.CC.Eval
+-- import Semantic.CC.Eval
 
-import Semantic.CC.Denotation
+-- import Semantic.CC.Denotation
 
 -- import Semantic.CC.Soundness
